src/Implementations/BlockAllocator/BlockAllocator.v
@@ -1,6 +1,8 @@
 Require Import Framework FSParameters TransactionalDiskLayer Omega.
 Import IfNotations.
-Close Scope pred_scope.
+Close Scope predicate_scope.
+
+Set Nested Proofs Allowed.
 
 Notation "| p |" := (Op (TransactionalDiskOperation data_length) p)(at level 60).
 Notation "x <-| p1 ; p2" := (Bind (Op (TransactionalDiskOperation data_length) p1) (fun x => p2))(right associativity, at level 60). 
@@ -52,6 +54,7 @@ Module Type BlockAllocatorParameters.
   Parameter bitmap_addr: addr.
   Parameter num_of_blocks: nat.
   Parameter num_of_blocks_in_bounds: num_of_blocks <= block_size.
+  Parameter blocks_fit_in_disk: bitmap_addr + num_of_blocks < data_length.
 End BlockAllocatorParameters.
   
 (* This is a generic block allocator which has a 1 block bitmap and num_of_blocks blocks following it *)  
@@ -113,9 +116,9 @@ Definition write a b :=
   else
     Ret None.
 
-Open Scope pred_scope.
+Open Scope predicate_scope.
   
-Fixpoint ptsto_bits' (dh: disk value) values bits n : @pred addr addr_dec value :=
+Fixpoint ptsto_bits' (dh: disk value) values bits n : @predicate addr addr_dec value :=
   match values, bits with
   | v::values', b::bits' =>
     (S n) |-> v *
@@ -131,11 +134,312 @@ Fixpoint ptsto_bits' (dh: disk value) values bits n : @pred addr addr_dec value 
       
 Definition ptsto_bits dh values bits := ptsto_bits' dh values bits 0.
 
-Definition block_allocator_rep (dh: disk value) : @pred addr addr_dec value  :=
+Definition block_allocator_rep (dh: disk value) : @predicate addr addr_dec value  :=
   (exists* bitmap values,
      let bits := bits (value_to_bits bitmap) in
      bitmap_addr |-> bitmap *
      ptsto_bits dh values bits *
      [[ length values = num_of_blocks ]] *
-     [[ forall i, i >= num_of_blocks -> dh i = None ]])%pred.
+     [[ forall i, i >= num_of_blocks -> dh i = None ]])%predicate.
+
+Print state'.
+
+Lemma ptsto_bits'_split:
+  forall dh a l1 l2 n,
+    a < length l1 ->
+    length l1 <= length l2 ->
+    ptsto_bits' dh l1 l2 n =*=> ptsto_bits' dh (firstn a l1) (firstn a l2) n * ptsto_bits' dh (skipn a l1) (skipn a l2) (n + a).
+Proof.
+  induction a; simpl; intros; eauto.
+  rewrite Nat.add_0_r; eauto.
+  cancel.
+  destruct l1; simpl in *; try omega.
+  destruct l2; simpl in *; try omega.
+  cancel.
+  rewrite <- Nat.add_succ_comm.
+  eapply IHa; omega.
+Qed.
+
+Lemma ptsto_bits'_merge:
+  forall dh a l1 l2 n,
+    a < length l1 ->
+    length l1 <= length l2 ->
+    ptsto_bits' dh (firstn a l1) (firstn a l2) n * ptsto_bits' dh (skipn a l1) (skipn a l2) (n + a) =*=>
+    ptsto_bits' dh l1 l2 n.
+Proof.
+  induction a; simpl; intros; eauto.
+  rewrite Nat.add_0_r; eauto.
+  cancel.
+  destruct l1; simpl in *; try omega.
+  destruct l2; simpl in *; try omega.
+  cancel.
+  rewrite <- Nat.add_succ_comm.
+  eapply pimpl_trans; [| eapply IHa; omega].
+  cancel.  
+Qed.
+
+Lemma ptsto_bits_extract :
+  forall dh values bits n,
+    n < length values ->
+    length values <= length bits ->
+    ptsto_bits dh values bits =*=> (S n |-> (selN values n value0) --* ptsto_bits dh values bits) * (S n |-> (selN values n value0)).
+Proof.
+  intros.
+  eapply septract_sep_star_extract.
+  unfold ptsto_bits.
+  intros m Hm.
+  eapply ptsto_bits'_split in Hm; eauto; simpl in *.
+  destruct_fresh (skipn n values).
+  - apply length_zero_iff_nil in D.
+    rewrite skipn_length in D.
+    omega.
+  - destruct_fresh (skipn n bits0).
+    apply length_zero_iff_nil in D0.
+    rewrite skipn_length in D0.
+    omega.
+    simpl in *.
+    pred_apply; cancel. 
+   
+    rewrite <- Nat.add_0_r with (n:= n).
+    rewrite <- skipn_selN.
+    rewrite Nat.add_0_r with (n:= n).
+    rewrite D; simpl.
+    cancel.
+    eexists; pred_apply; cancel.
+Qed.
+
+
+(* Specs *)
+
+Open Scope predicate_scope.
+Theorem alloc_ok:
+  forall dh v t s' F,
+    (* (F * block_allocator_rep dh)%predicate m -> *)
+    strongest_postcondition (TransactionalDiskLang data_length) (alloc v)
+                            (fun o s => (F * block_allocator_rep dh)%predicate (mem_union (fst s) (snd s)) /\
+                                     (forall tok, In tok o -> tok <> OpOracle (TransactionalDiskOperation data_length) [TxnFull])%list ) t s' ->
+    (exists a, t = Some a /\ (F * block_allocator_rep (upd dh a v))%predicate (mem_union (fst s') (snd s'))) \/
+    (t = None /\ (F * block_allocator_rep dh)%predicate (mem_union (fst s') (snd s'))).
+Proof. (*
+  unfold block_allocator_rep; simpl; intros.
+  pose proof num_of_blocks_in_bounds.
+  pose proof blocks_fit_in_disk.
+  repeat (cleanup; simpl in * ).
+  repeat (split_ors; cleanup; simpl in * ); try omega;
+  try solve [ unfold not in *; exfalso; eapply H10; [| eauto]; eauto].
+                  
+  - left; eexists; intuition eauto.
+    destruct_lifts.
+    repeat rewrite mem_union_upd.
+    do 2 destruct H.
+    destruct_lifts.
+    do 2 eexists.
+    eapply pimpl_trans; [| eauto | eapply ptsto_upd].
+    2: {
+      eapply sep_star_assoc.
+      apply sep_star_comm.
+      eapply ptsto_upd.
+      apply sep_star_comm.
+      eapply sep_star_assoc.
+      pred_apply; cancel.
+      apply ptsto_bits_extract.
+      omega.
+      destruct (value_to_bits x); simpl in *.
+      unfold valid_bitlist in *; cleanup.
+      apply num_of_blocks_in_bounds.
+    }
+    cancel.
+    rewrite bits_to_value_to_bits; simpl.
+    instantiate (1:= updN x1 (get_first_zero (firstn num_of_blocks (bits (value_to_bits x0)))) v).
+    admit. (* Separation logic goal *)
+    rewrite length_updN; eauto.
+    rewrite upd_ne; eauto.
+    omega.
+
+  - left; eexists; intuition eauto.
+    destruct_lifts.
+    repeat rewrite mem_union_upd.
+    do 2 destruct H.
+    destruct_lifts.
+    do 2 eexists.
+    eapply pimpl_trans; [| eauto | eapply ptsto_upd].
+    2: {
+      eapply sep_star_assoc.
+      apply sep_star_comm.
+      eapply ptsto_upd.
+      apply sep_star_comm.
+      eapply sep_star_assoc.
+      pred_apply; cancel.
+      apply ptsto_bits_extract.
+      omega.
+      destruct (value_to_bits x); simpl in *.
+      unfold valid_bitlist in *; cleanup.
+      apply num_of_blocks_in_bounds.
+    }
+    cancel.
+    rewrite bits_to_value_to_bits; simpl.
+    instantiate (1:= updN x1 (get_first_zero (firstn num_of_blocks (bits (value_to_bits x0)))) v).
+    admit. (* Separation logic goal *)
+    rewrite length_updN; eauto.
+    rewrite upd_ne; eauto.
+    omega.
+    
+  -
+    split_ors; cleanup; try omega.
+    right; intuition eauto.
+    *)
+Admitted.
+
+
+Theorem free_ok:
+  forall dh a t s' F,
+    strongest_postcondition (TransactionalDiskLang data_length) (free a)
+                            (fun o s => (F * block_allocator_rep dh)%predicate (mem_union (fst s) (snd s)) /\
+                                     (forall tok, In tok o -> tok <> OpOracle (TransactionalDiskOperation data_length) [TxnFull])%list ) t s' ->
+    (t = Some tt /\ (F * block_allocator_rep (delete dh a))%predicate (mem_union (fst s') (snd s'))) \/
+    (t = None /\ (F * block_allocator_rep dh)%predicate (mem_union (fst s') (snd s'))).
+Proof. (*
+  unfold block_allocator_rep; simpl; intros.
+  pose proof num_of_blocks_in_bounds.
+  pose proof blocks_fit_in_disk.
+  unfold free in *.
+  repeat (cleanup; simpl in * ); try omega;
+  repeat (split_ors; cleanup; simpl in * ); try omega;
+  try solve [ unfold not in *; exfalso; eapply H8; [| eauto]; eauto];
+  try solve [ unfold not in *; exfalso; eapply H9; [| eauto]; eauto];
+  try solve [right; intuition eauto].
+          
+  - left; eexists; intuition eauto.
+    destruct_lifts.
+    repeat rewrite mem_union_upd.
+    do 2 destruct H.
+    destruct_lifts.
+    do 2 eexists.
+    eapply ptsto_upd in H.
+    pred_apply' H.
+    cancel.
+    rewrite bits_to_value_to_bits; simpl.
+    instantiate (1:= x1).
+    admit. (* Separation logic goal *)
+    eauto.
+    unfold delete.
+    destruct (addr_dec i a); eauto.
+
+  - left; eexists; intuition eauto.
+    destruct_lifts.
+    repeat rewrite mem_union_upd.
+    do 2 destruct H.
+    destruct_lifts.
+    do 2 eexists.
+    eapply ptsto_upd in H.
+    pred_apply' H.
+    cancel.
+    rewrite bits_to_value_to_bits; simpl.
+    instantiate (1:= x1).
+    admit. (* Separation logic goal *)
+    eauto.
+    unfold delete.
+    destruct (addr_dec i a); eauto.
+*)
+Admitted.
+
+
+Theorem read_ok:
+  forall dh a t s' F,
+    strongest_postcondition (TransactionalDiskLang data_length) (read a)
+                            (fun o s => (F * block_allocator_rep dh)%predicate (mem_union (fst s) (snd s))) t s' ->
+    (t = dh a /\ (F * block_allocator_rep dh)%predicate (mem_union (fst s') (snd s'))).
+Proof. (*
+  unfold block_allocator_rep; simpl; intros.
+  pose proof num_of_blocks_in_bounds.
+  pose proof blocks_fit_in_disk.
+  unfold read in *.
+  repeat (cleanup; simpl in * ); try omega;
+  repeat (split_ors; cleanup; simpl in * ); eauto; try omega.
+*)
+Admitted.
+
+
+Theorem write_ok:
+  forall dh a v t s' F,
+    strongest_postcondition (TransactionalDiskLang data_length) (write a v)
+                            (fun o s => (F * block_allocator_rep dh)%predicate (mem_union (fst s) (snd s)) /\
+                                     (forall tok, In tok o -> tok <> OpOracle (TransactionalDiskOperation data_length) [TxnFull])%list ) t s' ->
+    (exists v', dh a = Some v' /\ t = Some tt /\ (F * block_allocator_rep (upd dh a v))%predicate (mem_union (fst s') (snd s'))) \/
+    (t = None /\ (F * block_allocator_rep dh)%predicate (mem_union (fst s') (snd s'))).
+Proof. (*
+  unfold block_allocator_rep; simpl; intros.
+  pose proof num_of_blocks_in_bounds.
+  pose proof blocks_fit_in_disk.
+  unfold write in *.
+  repeat (cleanup; simpl in * ); try omega;
+  repeat (split_ors; cleanup; simpl in * ); try omega;
+  try solve [ unfold not in *; exfalso; eapply H8; [| eauto]; eauto];
+  try solve [ unfold not in *; exfalso; eapply H9; [| eauto]; eauto];
+  try solve [right; intuition eauto].
+          
+  - left; eexists; intuition eauto.
+    destruct_lifts.
+    repeat rewrite mem_union_upd.
+    do 2 destruct H.
+    destruct_lifts.
+    do 2 eexists.
+      eapply pimpl_trans; [| eauto | eapply ptsto_upd].
+    2: {
+      eapply sep_star_assoc.
+      apply sep_star_comm.
+      pred_apply; cancel.
+      instantiate (3:= bitmap_addr|-> x).
+      cancel.
+      intros m Hm.
+     
+      apply sep_star_comm.
+      pred_apply. apply ptsto_bits_extract.
+      omega.
+      destruct (value_to_bits x); simpl in *.
+      unfold valid_bitlist in *; cleanup.
+      apply num_of_blocks_in_bounds.
+    }
+    cancel.
+    instantiate (1:= updN x1 a v).
+    admit. (* Separation logic goal *)
+    rewrite length_updN; eauto. 
+    rewrite upd_ne; eauto.
+    omega.
+
+  - left; eexists; intuition eauto.
+    destruct_lifts.
+    repeat rewrite mem_union_upd.
+    do 2 destruct H.
+    destruct_lifts.
+    do 2 eexists.
+      eapply pimpl_trans; [| eauto | eapply ptsto_upd].
+    2: {
+      eapply sep_star_assoc.
+      apply sep_star_comm.
+      pred_apply; cancel.
+      instantiate (3:= bitmap_addr|-> x).
+      cancel.
+      intros m Hm.
+     
+      apply sep_star_comm.
+      pred_apply. apply ptsto_bits_extract.
+      omega.
+      destruct (value_to_bits x); simpl in *.
+      unfold valid_bitlist in *; cleanup.
+      apply num_of_blocks_in_bounds.
+    }
+    cancel.
+    instantiate (1:= updN x1 a v).
+    admit. (* Separation logic goal *)
+    rewrite length_updN; eauto. 
+    rewrite upd_ne; eauto.
+    omega.
+*)
+Admitted.
+
+Global Opaque alloc free read write.
+
 End BlockAllocator.
+
+
