src/Implementations/FSParameters/FSParameters.v
@@ -1,4 +1,4 @@
-Require Import Framework.
+Require Import Framework Omega.
 
 Axiom block_size: nat.
 Axiom disk_size: nat.
@@ -11,17 +11,33 @@ Axiom log_length : nat.
 Definition data_start := 2 + log_length.
 Definition data_length := disk_size - data_start.
 
-(* Below all reside in data region *)
+(* Below all reside in data region indexed accordingly *)
 (* For simplicity, it will be 1 inode per block *)
-Definition inode_blocks_start := data_start.
+Definition inode_blocks_start := 0.
 Axiom inode_count: nat.
 Axiom inode_count_in_bounds: inode_count <= block_size.
 
-Definition file_blocks_start:= S(data_start + inode_count). (* 1 bitmap + inode_count inodes *)
+Definition file_blocks_start:= S(inode_count). (* 1 bitmap + inode_count inodes *)
 Axiom file_blocks_count : nat.
 Axiom file_blocks_count_in_bounds: file_blocks_count <= block_size.
 
 Axiom all_fits_to_data_region : 2 + inode_count + file_blocks_count <= data_length.
+
+Theorem inodes_fit_in_disk:
+  inode_blocks_start + inode_count < data_length.
+Proof.
+  pose proof all_fits_to_data_region.
+  unfold inode_blocks_start.
+  omega.
+Qed.
+
+Theorem file_blocks_fit_in_disk:
+  file_blocks_start + file_blocks_count < data_length.
+Proof.
+  pose proof all_fits_to_data_region.
+  unfold file_blocks_start.
+  omega.
+Qed.
 
 Axiom addr_list_to_blocks : list addr -> list value.
 
