src/Implementations/File/File.v
@@ -1,12 +1,13 @@
 Require Import Framework FSParameters AuthenticatedDiskLayer BlockAllocator Inode.
 Import IfNotations.
 
-Open Scope pred_scope.
+Open Scope predicate_scope.
 
 Module DiskAllocatorParams <: BlockAllocatorParameters.
   Definition bitmap_addr := file_blocks_start.
   Definition num_of_blocks := file_blocks_count.
   Definition num_of_blocks_in_bounds := file_blocks_count_in_bounds.
+  Definition blocks_fit_in_disk := file_blocks_fit_in_disk.
 End DiskAllocatorParams.
 
 Module DiskAllocator := BlockAllocator DiskAllocatorParams.
@@ -24,8 +25,8 @@ Definition file_rep (file: File) (inode: Inode) (file_block_map: disk value) :=
        nth_error inode.(block_numbers) i = Some block_number ->
        nth_error file.(blocks) i = file_block_map block_number).
 
-Definition files_inner_rep file_map inode_map file_block_map :=
-   addrs_match file_map inode_map /\
+Definition files_inner_rep (file_map: @mem Inum addr_dec File) inode_map file_block_map :=
+   addrs_match_exactly file_map inode_map /\
    (forall inum inode file,
      inode_map inum  = Some inode ->
      file_map inum = Some file ->
@@ -141,3 +142,441 @@ Definition create owner :=
   else
     _ <- |ADDO| Abort;
     Ret None.
+
+
+
+Theorem sp_lift1_ok:
+  forall O1 O2 (L1 : Language O1) (L2: Language O2) (HL: Language (HorizontalComposition O1 O2))
+    T (p: prog L1 T) s t P,
+    strongest_postcondition HL (lift_L1 O2 p) P t s ->
+    strongest_postcondition L1 p (fun o sx => P (map (fun o' =>
+                                                     match o' with
+                                                     |OpOracle _ o1 =>
+                                                      OpOracle (HorizontalComposition O1 O2) [Oracle1 O1 O2 o1]%list
+                                                     |Language.Cont _ =>
+                                                      Language.Cont _
+                                                     |Language.Crash _ =>
+                                                      Language.Crash _
+                                                     end) o) (sx, snd s)) t (fst s).
+Proof.
+  induction p; destruct s; simpl in *; intros; cleanup; eauto.
+  eapply H in H0; simpl in *.
+  eapply sp_to_exec in H0; cleanup.
+  eapply IHp in H1; simpl in *.
+  setoid_rewrite <- map_app in H1.
+  exists x; intuition eauto.
+  eapply exec_to_sp; eauto.
+Qed.
+
+Theorem sp_lift2_ok:
+  forall O1 O2 (L1 : Language O1) (L2: Language O2) (HL: Language (HorizontalComposition O1 O2))
+    T (p: prog L2 T) s t P,
+    strongest_postcondition HL (lift_L2 O1 p) P t s ->
+    strongest_postcondition L2 p (fun o sx => P (map (fun o' =>
+                                                     match o' with
+                                                     |OpOracle _ o2 =>
+                                                      OpOracle (HorizontalComposition O1 O2) [Oracle2 O1 O2 o2]%list
+                                                     |Language.Cont _ =>
+                                                      Language.Cont _
+                                                     |Language.Crash _ =>
+                                                      Language.Crash _
+                                                     end) o) (fst s, sx)) t (snd s).
+Proof.
+  induction p; destruct s; simpl in *; intros; cleanup; eauto.
+  eapply H in H0; simpl in *.
+  eapply sp_to_exec in H0; cleanup.
+  eapply IHp in H1; simpl in *.
+  setoid_rewrite <- map_app in H1.
+  exists x; intuition eauto.
+  eapply exec_to_sp; eauto.
+Qed.
+
+Theorem sp_extract_precondition:
+  forall O (L : Language O) T (p: prog L T) s t P,
+    strongest_postcondition L p P t s ->
+    strongest_postcondition L p P t s /\ (exists o s, P o s).
+Proof.
+  intros; eapply_fresh sp_to_exec in H; cleanup; eauto.
+Qed.
+
+Theorem auth_then_exec_ok:
+  forall inum T (p: Inum -> prog (TransactionalDiskLang data_length) (option T)) s' t fmap F (Q: option T -> state  (TransactionalDiskLang data_length) -> Prop),
+    
+    (forall fmap' t' s'',
+       strongest_postcondition (TransactionalDiskLang data_length) (p inum)
+                               (fun o s => (F * files_rep fmap')%predicate (mem_union (fst s) (snd s))) t' s'' ->
+       (t' = None /\ Q t' (empty_mem, snd s'')) \/
+       (t' <> None /\ Q t' (empty_mem, mem_union (fst s'') (snd s'')))) -> 
+    (strongest_postcondition AuthenticatedDiskLang (auth_then_exec inum p)
+     (fun o s => (F * files_rep fmap)%predicate (mem_union (fst (snd s)) (snd (snd s))) /\ (fst (snd s)) = empty_mem) t s' ->
+     (exists file, fmap inum = Some file /\ fst s' = file.(owner) /\ fst (snd s') = empty_mem /\ Q t (snd s')) \/
+    (fst (snd s') = empty_mem /\ (fmap inum = None \/ (exists file, fmap inum = Some file /\ fst s' <> file.(owner))))).
+Proof.
+  unfold auth_then_exec; intros.
+  apply sp_bind in H0; simpl in *.
+  cleanup; simpl in *.
+  {(* Valid inum *)
+    cleanup; simpl in *.
+    { (* Auth success *)
+      cleanup; simpl in *.
+      cleanup; simpl in *.
+      { (* After p *)
+        cleanup; simpl in *.
+        cleanup; simpl in *.
+        { (* p success *)
+          cleanup; simpl in *.
+          repeat (apply sp_exists_extract in H1; cleanup).
+          apply sp_lift2_ok in H1; simpl in H1.
+          apply sp_extract_precondition in H1; cleanup.
+          repeat (apply sp_exists_extract in H2; cleanup).
+          split_ors; cleanup.
+          apply sp_lift2_ok in H2; simpl in H2; cleanup.
+          
+          eapply sp_impl in H2.
+          apply (sp_exists_extract (disk Inode)) with
+          (P:= fun (inode_map: disk Inode) o (sx : state') => (F *
+           (exists* (file_block_map : disk value),
+            inode_rep inode_map * DiskAllocator.block_allocator_rep file_block_map *
+            [[files_inner_rep fmap inode_map file_block_map]]))%predicate (mem_union (fst sx) (snd sx)) /\
+                                                           tt = tt /\ sx = (empty_mem, snd x0)) in H2; cleanup.
+
+          2: {
+            simpl; intros; cleanup.            
+            unfold files_rep in H5.
+            apply pimpl_exists_l_star_r in H5.
+            destruct H5.
+            exists x6; simpl; eauto.
+          }
+          
+          eapply sp_impl in H2.
+          apply (sp_exists_extract (disk value)) with
+          (P:= fun (file_block_map: disk value) o (sx : state') => (F *
+           (inode_rep x6 * DiskAllocator.block_allocator_rep file_block_map *
+            [[files_inner_rep fmap x6 file_block_map]]))%predicate (mem_union (fst sx) (snd sx)) /\
+                                                           tt = tt /\ sx = (empty_mem, snd x0)) in H2; cleanup.
+
+          2: {
+            simpl; intros; cleanup.            
+            apply pimpl_exists_l_star_r in H5.
+            destruct H5.
+            exists x7; simpl; eauto.
+          }
+          
+          apply sp_extract_precondition in H2; cleanup.
+          simpl in *.
+          eapply sp_impl in H2.
+          apply get_owner_ok in H2.
+          
+          2: {
+            simpl; intros; cleanup.
+            simpl in *.
+            instantiate (1:= x6).
+            instantiate (1:= (F * DiskAllocator.block_allocator_rep x7 * [[files_inner_rep fmap x6 x7]])).
+            pred_apply; cancel.
+          }
+          
+          split_ors; cleanup.
+          destruct_lifts; cleanup.
+          unfold files_inner_rep in *; cleanup.
+          specialize (H4 inum).
+          destruct_fresh (fmap inum); intuition eauto.
+          
+          left; eexists; intuition eauto.
+          specialize H8 with (1:= H2)(2:=D).
+          unfold file_rep in *; cleanup; eauto.
+          eapply sp_impl in H1; eauto.
+          eapply H in H1; simpl in *; eauto.
+          split_ors; cleanup; eauto.
+
+          intros; simpl in *; cleanup.
+          apply sp_lift2_ok in H4; simpl in H4; cleanup.
+
+          eapply sp_impl in H4.
+          apply (sp_exists_extract (disk Inode)) with
+          (P:= fun (inode_map: disk Inode) o (sx : state') => (F *
+           (exists* (file_block_map : disk value),
+            inode_rep inode_map * DiskAllocator.block_allocator_rep file_block_map *
+            [[files_inner_rep fmap inode_map file_block_map]]))%predicate (mem_union (fst sx) (snd sx))) in H4; cleanup.
+
+          2: {
+            simpl; intros; cleanup.            
+            unfold files_rep in H12.
+            apply pimpl_exists_l_star_r in H12.
+            destruct H12.
+            exists x1; simpl; eauto.
+          }
+          
+          eapply sp_impl in H4.
+          apply (sp_exists_extract (disk value)) with
+          (P:= fun (file_block_map: disk value) o (sx : state') => (F *
+           (inode_rep x0 * DiskAllocator.block_allocator_rep file_block_map *
+            [[files_inner_rep fmap x0 file_block_map]]))%predicate (mem_union (fst sx) (snd sx))) in H4; cleanup.
+
+          2: {
+            simpl; intros; cleanup.            
+            apply pimpl_exists_l_star_r in H12.
+            destruct H12.
+            exists x1; simpl in *; eauto.
+          }
+          
+          
+          apply sp_extract_precondition in H4; cleanup.
+          simpl in *.
+          eapply sp_impl in H4.
+          apply get_owner_ok in H4.
+          split_ors; cleanup.
+
+          2: {
+            simpl; intros; cleanup.
+            simpl in *.
+            instantiate (1:= x0).
+            instantiate (1:= (F * DiskAllocator.block_allocator_rep x1 * [[files_inner_rep fmap x0 x1]])).
+            pred_apply; cancel.
+          }
+
+          unfold files_rep.         
+          apply sep_star_comm.
+          repeat apply pimpl_exists_r_star.
+          exists x0.
+          apply pimpl_exists_r_star.
+          exists x1.
+          pred_apply; cancel.
+          all: exact AuthenticationLang.
+        }
+        { (* p Failed. *)
+          cleanup; simpl in *.
+          repeat (apply sp_exists_extract in H1; cleanup).
+          apply sp_lift2_ok in H1; simpl in H1.
+          apply sp_extract_precondition in H1; cleanup.
+          repeat (apply sp_exists_extract in H2; cleanup).
+          split_ors; cleanup.
+          apply sp_lift2_ok in H2; simpl in H2; cleanup.
+          
+          eapply sp_impl in H2.
+          apply (sp_exists_extract (disk Inode)) with
+          (P:= fun (inode_map: disk Inode) o (sx : state') => (F *
+           (exists* (file_block_map : disk value),
+            inode_rep inode_map * DiskAllocator.block_allocator_rep file_block_map *
+            [[files_inner_rep fmap inode_map file_block_map]]))%predicate (mem_union (fst sx) (snd sx)) /\
+                                                           tt = tt /\ sx = (empty_mem, snd x0)) in H2; cleanup.
+
+          2: {
+            simpl; intros; cleanup.            
+            unfold files_rep in H5.
+            apply pimpl_exists_l_star_r in H5.
+            destruct H5.
+            exists x6; simpl; eauto.
+          }
+          
+          eapply sp_impl in H2.
+          apply (sp_exists_extract (disk value)) with
+          (P:= fun (file_block_map: disk value) o (sx : state') => (F *
+           (inode_rep x6 * DiskAllocator.block_allocator_rep file_block_map *
+            [[files_inner_rep fmap x6 file_block_map]]))%predicate (mem_union (fst sx) (snd sx)) /\
+                                                           tt = tt /\ sx = (empty_mem, snd x0)) in H2; cleanup.
+
+          2: {
+            simpl; intros; cleanup.            
+            apply pimpl_exists_l_star_r in H5.
+            destruct H5.
+            exists x7; simpl; eauto.
+          }
+          
+          apply sp_extract_precondition in H2; cleanup.
+          simpl in *.
+          eapply sp_impl in H2.
+          apply get_owner_ok in H2.
+          
+          2: {
+            simpl; intros; cleanup.
+            simpl in *.
+            instantiate (1:= x6).
+            instantiate (1:= (F * DiskAllocator.block_allocator_rep x7 * [[files_inner_rep fmap x6 x7]])).
+            pred_apply; cancel.
+          }
+          
+          split_ors; cleanup.
+          destruct_lifts; cleanup.
+          unfold files_inner_rep in *; cleanup.
+          specialize (H4 inum).
+          destruct_fresh (fmap inum); intuition eauto.
+          
+          left; eexists; intuition eauto.
+          specialize H8 with (1:= H2)(2:=D).
+          unfold file_rep in *; cleanup; eauto.
+          eapply sp_impl in H1; eauto.
+          eapply H in H1; simpl in *; eauto.        
+          split_ors; cleanup; intuition eauto.
+          
+          simpl; intros; cleanup.
+          repeat (apply sp_exists_extract in H4; cleanup).
+          apply sp_lift2_ok in H4; simpl in H4; cleanup.
+
+          eapply sp_impl in H4.
+          apply (sp_exists_extract (disk Inode)) with
+          (P:= fun (inode_map: disk Inode) o (sx : state') => (F *
+           (exists* (file_block_map : disk value),
+            inode_rep inode_map * DiskAllocator.block_allocator_rep file_block_map *
+            [[files_inner_rep fmap inode_map file_block_map]]))%predicate (mem_union (fst sx) (snd sx)) /\
+                                                           tt = tt /\ sx = (empty_mem, snd x0)) in H4; cleanup.
+
+          2: {
+            simpl; intros; cleanup.            
+            unfold files_rep in H12.
+            apply pimpl_exists_l_star_r in H12.
+            destruct H12.
+            exists x1; simpl; eauto.
+          }
+          
+          eapply sp_impl in H4.
+          apply (sp_exists_extract (disk value)) with
+          (P:= fun (file_block_map: disk value) o (sx : state') => (F *
+           (inode_rep x1 * DiskAllocator.block_allocator_rep file_block_map *
+            [[files_inner_rep fmap x1 file_block_map]]))%predicate (mem_union (fst sx) (snd sx)) /\
+                                                           tt = tt /\ sx = (empty_mem, snd x0)) in H4; cleanup.
+
+          2: {
+            simpl; intros; cleanup.            
+            apply pimpl_exists_l_star_r in H12.
+            destruct H12.
+            exists x2; simpl in *; eauto.
+          }
+          
+          
+          apply sp_extract_precondition in H4; cleanup.
+          simpl in *.
+          eapply sp_impl in H4.
+          apply get_owner_ok in H4.
+          split_ors; cleanup.
+
+          2: {
+            simpl; intros; cleanup.
+            simpl in *.
+            instantiate (1:= x1).
+            instantiate (1:= (F * DiskAllocator.block_allocator_rep x2 * [[files_inner_rep fmap x1 x2]])).
+            pred_apply; cancel.
+          }
+
+          unfold files_rep.         
+          apply sep_star_comm.
+          repeat apply pimpl_exists_r_star.
+          exists x1.
+          apply pimpl_exists_r_star.
+          exists x2.
+          pred_apply; cancel.
+          all: exact AuthenticationLang.
+        }
+      }
+      { (* Auth Fail *)
+        simpl in *; cleanup.
+        split_ors; cleanup.
+
+        apply sp_lift2_ok in H1; simpl in H1; cleanup.        
+        repeat (apply sp_exists_extract in H1; cleanup).
+        eapply sp_impl in H1.
+          apply (sp_exists_extract (disk Inode)) with
+          (P:= fun (inode_map: disk Inode) o (sx : state') => (F *
+           (exists* (file_block_map : disk value),
+            inode_rep inode_map * DiskAllocator.block_allocator_rep file_block_map *
+            [[files_inner_rep fmap inode_map file_block_map]]))%predicate (mem_union (fst sx) (snd sx))) in H1; cleanup.
+
+          2: {
+            simpl; intros; cleanup.            
+            unfold files_rep in H5.
+            apply pimpl_exists_l_star_r in H5.
+            destruct H5.
+            exists x4; simpl; eauto.
+          }
+          
+          eapply sp_impl in H1.
+          apply (sp_exists_extract (disk value)) with
+          (P:= fun (file_block_map: disk value) o (sx : state') => (F *
+           (inode_rep x4 * DiskAllocator.block_allocator_rep file_block_map *
+            [[files_inner_rep fmap x4 file_block_map]]))%predicate (mem_union (fst sx) (snd sx))) in H1; cleanup.
+
+          2: {
+            simpl; intros; cleanup.            
+            apply pimpl_exists_l_star_r in H5.
+            destruct H5.
+            exists x0; simpl; eauto.
+          }
+          
+          eapply sp_impl in H1.
+          apply get_owner_ok in H1.
+          
+          2: {
+            simpl; intros; cleanup.
+            simpl in *.
+            instantiate (1:= x4).
+            instantiate (1:= (F * DiskAllocator.block_allocator_rep x0 * [[files_inner_rep fmap x4 x0]])).
+            pred_apply; cancel.
+          }
+          
+          split_ors; cleanup.
+          destruct_lifts; cleanup.
+          unfold files_inner_rep in *; cleanup.
+          specialize (H4 inum).
+          destruct_fresh (fmap inum); intuition eauto.
+          
+          right; intuition eauto.
+          specialize H7 with (1:= H1)(2:=D).
+          unfold file_rep in *; cleanup; eauto.
+          right; eexists; intuition eauto.
+          apply H2; cleanup; eauto.
+          all: exact AuthenticationLang.
+      }
+    }
+    { (* Invalid Inum *)
+      cleanup; simpl in *.
+       apply sp_lift2_ok in H1; simpl in H1; cleanup.        
+       repeat (apply sp_exists_extract in H1; cleanup).
+       eapply sp_impl in H1.
+       apply (sp_exists_extract (disk Inode)) with
+          (P:= fun (inode_map: disk Inode) o (sx : state') => (F *
+           (exists* (file_block_map : disk value),
+            inode_rep inode_map * DiskAllocator.block_allocator_rep file_block_map *
+            [[files_inner_rep fmap inode_map file_block_map]]))%predicate (mem_union (fst sx) (snd sx))) in H1; cleanup.
+
+          2: {
+            simpl; intros; cleanup.            
+            unfold files_rep in H2.
+            apply pimpl_exists_l_star_r in H2.
+            destruct H2.
+            exists x4; simpl; eauto.
+          }
+          
+          eapply sp_impl in H1.
+          apply (sp_exists_extract (disk value)) with
+          (P:= fun (file_block_map: disk value) o (sx : state') => (F *
+           (inode_rep x4 * DiskAllocator.block_allocator_rep file_block_map *
+            [[files_inner_rep fmap x4 file_block_map]]))%predicate (mem_union (fst sx) (snd sx))) in H1; cleanup.
+
+          2: {
+            simpl; intros; cleanup.            
+            apply pimpl_exists_l_star_r in H2.
+            destruct H2.
+            exists x0; simpl; eauto.
+          }
+          
+          eapply sp_impl in H1.
+          apply get_owner_ok in H1.
+          
+          2: {
+            simpl; intros; cleanup.
+            simpl in *.
+            instantiate (1:= x4).
+            instantiate (1:= (F * DiskAllocator.block_allocator_rep x0 * [[files_inner_rep fmap x4 x0]])).
+            pred_apply; cancel.
+          }
+          
+          split_ors; cleanup.
+          destruct_lifts; cleanup.
+          unfold files_inner_rep in *; cleanup.
+          specialize (H4 inum).
+          destruct_fresh (fmap inum); intuition eauto.
+
+          exfalso; apply H7; intuition eauto; congruence.
+          all: exact AuthenticationLang.
+    }      
+  }
+Qed.
