src/Implementations/Inode/Inode.v
@@ -1,4 +1,3 @@
-Require Import Transaction. (* Needed for extraction *)
 Require Import Framework FSParameters TransactionalDiskLayer BlockAllocator.
 Import IfNotations.
 
@@ -18,23 +17,24 @@ Axiom inode_encode_decode:
 Axiom inode_decode_encode:
   forall b,
     encode_inode (decode_inode b) = b.
-
+  
 Module InodeAllocatorParams <: BlockAllocatorParameters.
   Definition bitmap_addr := inode_blocks_start.
   Definition num_of_blocks := inode_count.
   Definition num_of_blocks_in_bounds := inode_count_in_bounds.
+  Definition blocks_fit_in_disk := inodes_fit_in_disk.
 End InodeAllocatorParams.
 
 Module InodeAllocator := BlockAllocator InodeAllocatorParams.
 
 Import InodeAllocator.
 
-Open Scope pred_scope.
+Open Scope predicate_scope.
 
 Definition inode_map_rep inode_block_map (inode_map: disk Inode) :=
   forall i, inode_map i = option_map decode_inode (inode_block_map i).
 
-Definition inode_rep (inode_map: disk Inode) : @pred addr addr_dec value :=
+Definition inode_rep (inode_map: disk Inode) : @predicate addr addr_dec value :=
   exists* inode_block_map,
     block_allocator_rep inode_block_map *
     [[ forall i, inode_map i = option_map decode_inode (inode_block_map i) ]].
@@ -94,3 +94,388 @@ Definition get_owner inum :=
     Ret (Some inode.(owner))
   else
     Ret None.
+
+
+Theorem get_inode_ok:
+  forall inum s' t imap F,
+    strongest_postcondition (TransactionalDiskLang data_length) (get_inode inum)
+                            (fun o s => (F * inode_rep imap)%predicate (mem_union (fst s) (snd s))) t s' ->
+    (t = imap inum /\ (F * inode_rep imap)%predicate (mem_union (fst s') (snd s'))).
+Proof.
+  unfold inode_rep; intros; simpl in *; cleanup.
+  destruct x; simpl in *; cleanup.
+  -    
+    eapply sp_impl in H.
+    eapply (sp_exists_extract (disk value)) with (P:=fun inode_block_map o s =>  (F *
+   (block_allocator_rep inode_block_map *
+    [[forall i : addr, imap i = option_map decode_inode (inode_block_map i)]]))%predicate
+    (mem_union (fst s) (snd s))) in H.
+    cleanup.
+    eapply sp_impl in H.
+    apply read_ok in H.
+    2: {
+      intros; cleanup.
+      simpl; eauto.
+      instantiate (1:= x).
+      instantiate (1:= F * [[forall i : addr, imap i = option_map decode_inode (x i)]]).
+      pred_apply' H0; cancel.
+    }
+    
+    cleanup.
+    destruct_lift H0.
+    rewrite H4; cleanup.
+    rewrite <- H; simpl.
+    intuition eauto.
+    pred_apply; cancel.
+    exists x; pred_apply; cancel.
+
+    simpl; intros; cleanup.
+    apply pimpl_exists_l_star_r in H0.
+    destruct H0.
+    exists x; eauto.
+    
+  -
+    eapply sp_impl in H.
+    eapply (sp_exists_extract (disk value)) with (P:=fun inode_block_map o s =>  (F *
+   (block_allocator_rep inode_block_map *
+    [[forall i : addr, imap i = option_map decode_inode (inode_block_map i)]]))%predicate
+    (mem_union (fst s) (snd s))) in H.
+    cleanup.
+    eapply sp_impl in H.
+    apply read_ok in H.
+    2: {
+      intros; cleanup.
+      simpl; eauto.
+      instantiate (1:= x).
+      instantiate (1:= F * [[forall i : addr, imap i = option_map decode_inode (x i)]]).
+      pred_apply' H0; cancel.
+    }
+    
+    cleanup.
+    destruct_lift H0.
+    rewrite H4; cleanup.
+    rewrite <- H; simpl.
+    intuition eauto.
+    pred_apply; cancel.
+    exists x; pred_apply; cancel.
+
+    simpl; intros; cleanup.
+    apply pimpl_exists_l_star_r in H0.
+    destruct H0.
+    exists x; eauto.
+Qed.
+
+
+Theorem set_inode_ok:
+  forall inum inode s' t imap F,
+    strongest_postcondition (TransactionalDiskLang data_length) (set_inode inum inode)
+                            (fun o s => (F * inode_rep imap)%predicate (mem_union (fst s) (snd s)) /\
+                            (forall tok, In tok o -> tok <> OpOracle (TransactionalDiskOperation data_length) [TxnFull])%list ) t s' ->
+    (exists i, imap inum = Some i /\ t = Some tt /\ (F * inode_rep (upd imap inum inode))%predicate (mem_union (fst s') (snd s'))) \/
+    (t = None /\ (F * inode_rep imap)%predicate (mem_union (fst s') (snd s'))).
+Proof.
+  unfold inode_rep; intros; simpl in *; cleanup.
+  eapply sp_impl in H.
+  eapply (sp_exists_extract (disk value)) with (P:=fun inode_block_map o s =>  (F *
+   (block_allocator_rep inode_block_map *
+    [[forall i : addr, imap i = option_map decode_inode (inode_block_map i)]]))%predicate
+                                                                          (mem_union (fst s) (snd s)) /\
+                                               (forall tok, In tok o -> tok <> OpOracle (TransactionalDiskOperation data_length) [TxnFull])%list) in H.
+    cleanup.
+    eapply sp_impl in H.
+    apply write_ok in H.
+    2: {
+      intros; cleanup.
+      simpl; eauto.
+      instantiate (1:= x0).
+      instantiate (1:= F * [[forall i : addr, imap i = option_map decode_inode (x0 i)]]).
+      split; eauto.
+      pred_apply' H0; cancel.
+    }
+    split_ors; cleanup.
+    
+  -    destruct_lift H1.
+    left; eexists; intuition eauto.
+    rewrite H4, H; simpl; eauto.
+    pred_apply; cancel.
+    exists (upd x0 inum (encode_inode inode)).
+    pred_apply; cancel.
+    destruct (addr_dec inum i); subst;
+    [ repeat rewrite upd_eq | repeat rewrite upd_ne]; simpl; eauto.
+    rewrite inode_encode_decode; eauto.
+
+  - right; intuition cleanup.
+    pred_apply; cancel.
+    exists x0.
+    pred_apply; cancel.
+    
+ - simpl; intros; cleanup.
+   apply pimpl_exists_l_star_r in H0.
+   destruct H0.
+   exists x0; eauto.
+Qed.
+
+Global Opaque get_inode set_inode.
+
+Theorem alloc_ok:
+  forall user s' t imap F,
+    strongest_postcondition (TransactionalDiskLang data_length) (alloc user)
+                            (fun o s => (F * inode_rep imap)%predicate (mem_union (fst s) (snd s)) /\
+                            (forall tok, In tok o -> tok <> OpOracle (TransactionalDiskOperation data_length) [TxnFull])%list ) t s' ->
+    (exists inum, t = Some inum /\ (F * inode_rep (upd imap inum (Build_Inode user [])))%predicate (mem_union (fst s') (snd s'))) \/
+    (t = None /\ (F * inode_rep imap)%predicate (mem_union (fst s') (snd s'))).
+Proof.
+    unfold inode_rep; intros; simpl in *; cleanup.
+  eapply sp_impl in H.
+  eapply (sp_exists_extract (disk value)) with (P:=fun inode_block_map o s =>  (F *
+   (block_allocator_rep inode_block_map *
+    [[forall i : addr, imap i = option_map decode_inode (inode_block_map i)]]))%predicate
+                                                                          (mem_union (fst s) (snd s)) /\
+                                               (forall tok, In tok o -> tok <> OpOracle (TransactionalDiskOperation data_length) [TxnFull])%list) in H.
+    cleanup.
+    eapply sp_impl in H.
+    apply alloc_ok in H.
+    2: {
+      intros; cleanup.
+      simpl; eauto.
+      instantiate (1:= x0).
+      instantiate (1:= F * [[forall i : addr, imap i = option_map decode_inode (x0 i)]]).
+      split; eauto.
+      pred_apply' H0; cancel.
+    }
+    split_ors; cleanup.
+  - left; exists x1; intuition cleanup.
+    pred_apply; cancel.
+    exists (upd x0 x1 (encode_inode (Build_Inode user []))).
+    pred_apply; cancel.
+    destruct (addr_dec x1 i); subst;
+    [ repeat rewrite upd_eq | repeat rewrite upd_ne]; simpl; eauto.
+    rewrite inode_encode_decode; eauto.
+    
+  - right; intuition cleanup.
+    pred_apply; cancel.
+    exists x0.
+    pred_apply; cancel.
+
+  - simpl; intros; cleanup.
+   apply pimpl_exists_l_star_r in H0.
+   destruct H0.
+   exists x0; eauto.    
+Qed.
+
+
+Theorem free_ok:
+  forall inum s' t imap F,
+    strongest_postcondition (TransactionalDiskLang data_length) (free inum)
+                            (fun o s => (F * inode_rep imap)%predicate (mem_union (fst s) (snd s)) /\
+                            (forall tok, In tok o -> tok <> OpOracle (TransactionalDiskOperation data_length) [TxnFull])%list ) t s' ->
+    (t = Some tt /\ (F * inode_rep (delete imap inum))%predicate (mem_union (fst s') (snd s'))) \/
+    (t = None /\ (F * inode_rep imap)%predicate (mem_union (fst s') (snd s'))).
+Proof.
+    unfold inode_rep; intros; simpl in *; cleanup.
+  eapply sp_impl in H.
+  eapply (sp_exists_extract (disk value)) with (P:=fun inode_block_map o s =>  (F *
+   (block_allocator_rep inode_block_map *
+    [[forall i : addr, imap i = option_map decode_inode (inode_block_map i)]]))%predicate
+                                                                          (mem_union (fst s) (snd s)) /\
+                                               (forall tok, In tok o -> tok <> OpOracle (TransactionalDiskOperation data_length) [TxnFull])%list) in H.
+    cleanup.
+    eapply sp_impl in H.
+    apply free_ok in H.
+    2: {
+      intros; cleanup.
+      simpl; eauto.
+      instantiate (1:= x0).
+      instantiate (1:= F * [[forall i : addr, imap i = option_map decode_inode (x0 i)]]).
+      split; eauto.
+      pred_apply' H0; cancel.
+    }
+    
+    split_ors; cleanup.
+  - left; intuition cleanup.
+    pred_apply; cancel.
+    exists (delete x0 inum).
+    pred_apply; cancel.
+    unfold delete.
+    destruct (addr_dec i inum); eauto.
+    
+  - right; intuition cleanup.
+    pred_apply; cancel.
+    exists x0.
+    pred_apply; cancel.
+
+  - simpl; intros; cleanup.
+   apply pimpl_exists_l_star_r in H0.
+   destruct H0.
+   exists x0; eauto.   
+Qed.
+
+Theorem extend_ok:
+  forall inum block_num s' t imap F,
+    strongest_postcondition (TransactionalDiskLang data_length) (extend inum block_num)
+                            (fun o s => (F * inode_rep imap)%predicate (mem_union (fst s) (snd s)) /\
+                            (forall tok, In tok o -> tok <> OpOracle (TransactionalDiskOperation data_length) [TxnFull])%list ) t s' ->
+    (exists inode, imap inum = Some inode /\ t = Some tt /\ (F * inode_rep (upd imap inum (Build_Inode inode.(owner) (inode.(block_numbers)++[block_num]))))%predicate (mem_union (fst s') (snd s'))) \/
+    (t = None /\ (F * inode_rep imap)%predicate (mem_union (fst s') (snd s'))).
+Proof.
+  unfold extend; intros; cleanup.
+  apply sp_bind in H.
+  simpl in *; cleanup.
+  
+  eapply sp_impl in H;
+  [> eapply get_inode_ok in H; eauto
+  |try solve [intros; cleanup; simpl; intuition eauto] ].
+  cleanup.
+
+  apply sp_bind in H0.
+  simpl in *; cleanup.
+  eapply sp_impl in H2;
+  [> eapply set_inode_ok in H2; eauto
+  |try solve [intros; cleanup; simpl; intuition eauto] ].  
+  split_ors; cleanup.
+  
+  + cleanup; left; eexists; intuition eauto.
+    cleanup; eauto.
+  + right; intuition eauto.
+  + simpl; intros.
+    eapply sp_impl in H3;
+    [> eapply get_inode_ok in H3; eauto
+    |].
+    instantiate (2:= F * [[forall tok, In tok o -> tok <> OpOracle (TransactionalDiskOperation data_length) [TxnFull]%list ]] ) in H3.
+    cleanup; destruct_lift H4.
+    split; eauto.
+
+    simpl; intros; cleanup.
+    pred_apply; cancel.
+    eapply H5; eauto.
+  + simpl in *; cleanup.
+    eapply sp_impl in H0;
+    [> eapply get_inode_ok in H0; eauto
+    |try solve [intros; cleanup; simpl; intuition eauto] ].
+    cleanup.
+    right; intuition.
+Qed.
+
+
+Theorem change_owner_ok:
+  forall inum user s' t imap F,
+    strongest_postcondition (TransactionalDiskLang data_length) (change_owner inum user)
+                            (fun o s => (F * inode_rep imap)%predicate (mem_union (fst s) (snd s)) /\
+                            (forall tok, In tok o -> tok <> OpOracle (TransactionalDiskOperation data_length) [TxnFull])%list ) t s' ->
+    (exists inode, imap inum = Some inode /\ t = Some tt /\ (F * inode_rep (upd imap inum (Build_Inode user (inode.(block_numbers)))))%predicate (mem_union (fst s') (snd s'))) \/
+    (t = None /\ (F * inode_rep imap)%predicate (mem_union (fst s') (snd s'))).
+Proof.
+  unfold change_owner; intros; cleanup.
+  apply sp_bind in H.
+  simpl in *; cleanup.
+  
+  eapply sp_impl in H;
+  [> eapply get_inode_ok in H; eauto
+  |try solve [intros; cleanup; simpl; intuition eauto] ].
+  cleanup.
+
+  apply sp_bind in H0.
+  simpl in *; cleanup.
+  eapply sp_impl in H2;
+  [> eapply set_inode_ok in H2; eauto
+  |try solve [intros; cleanup; simpl; intuition eauto] ].  
+  split_ors; cleanup.
+  
+  + cleanup; left; eexists; intuition eauto.
+    cleanup; eauto.
+  + right; intuition eauto.
+  + simpl; intros.
+    eapply sp_impl in H3;
+    [> eapply get_inode_ok in H3; eauto
+    |].
+    instantiate (2:= F * [[forall tok, In tok o -> tok <> OpOracle (TransactionalDiskOperation data_length) [TxnFull]%list ]] ) in H3.
+    cleanup; destruct_lift H4.
+    split; eauto.
+
+    simpl; intros; cleanup.
+    pred_apply; cancel.
+    eapply H5; eauto.
+  + simpl in *; cleanup.
+    eapply sp_impl in H0;
+    [> eapply get_inode_ok in H0; eauto
+    |try solve [intros; cleanup; simpl; intuition eauto] ].
+    cleanup.
+    right; intuition.
+Qed.
+
+Theorem get_block_number_ok:
+  forall inum off s' t imap F,
+    strongest_postcondition (TransactionalDiskLang data_length) (get_block_number inum off)
+                            (fun o s => (F * inode_rep imap)%predicate (mem_union (fst s) (snd s))) t s' ->
+    (exists inode, imap inum = Some inode /\ t = nth_error inode.(block_numbers) off /\ (F * inode_rep imap)%predicate (mem_union (fst s') (snd s'))) \/
+    (t = None /\ imap inum = None /\ (F * inode_rep imap)%predicate (mem_union (fst s') (snd s'))).
+Proof.
+  unfold get_block_number; intros; cleanup.
+  apply sp_bind in H.
+  simpl in *; cleanup.
+    
+  eapply sp_impl in H;
+  [> eapply get_inode_ok in H; eauto
+  |try solve [intros; cleanup; simpl; intuition eauto] ].
+  cleanup.
+  
+  + simpl in *; cleanup; left; eexists; intuition eauto.
+    eapply get_inode_ok in H0; eauto.
+    cleanup; eauto.
+  + simpl in *; cleanup; right; intuition eauto.
+    eapply get_inode_ok in H0; eauto.
+    cleanup; eauto.
+Qed.
+
+
+Theorem get_block_numbers_ok:
+  forall inum s' t imap F,
+    strongest_postcondition (TransactionalDiskLang data_length) (get_block_numbers inum)
+                            (fun o s => (F * inode_rep imap)%predicate (mem_union (fst s) (snd s))) t s' ->
+    (exists inode, imap inum = Some inode /\ t = Some inode.(block_numbers) /\ (F * inode_rep imap)%predicate (mem_union (fst s') (snd s'))) \/
+    (t = None /\ imap inum = None /\ (F * inode_rep imap)%predicate (mem_union (fst s') (snd s'))).
+Proof.
+  unfold get_block_numbers; intros; cleanup.
+  apply sp_bind in H.
+  simpl in *; cleanup.
+    
+  eapply sp_impl in H;
+  [> eapply get_inode_ok in H; eauto
+  |try solve [intros; cleanup; simpl; intuition eauto] ].
+  cleanup.
+  
+  + simpl in *; cleanup; left; eexists; intuition eauto.
+    eapply get_inode_ok in H0; eauto.
+    cleanup; eauto.
+    
+  + simpl in *; cleanup; right; intuition eauto.
+    eapply get_inode_ok in H0; eauto.
+    cleanup; eauto.
+Qed.
+
+Theorem get_owner_ok:
+  forall inum s' t imap F,
+    strongest_postcondition (TransactionalDiskLang data_length) (get_owner inum)
+                            (fun o s => (F * inode_rep imap)%predicate (mem_union (fst s) (snd s))) t s' ->
+    (exists inode, imap inum = Some inode /\ t = Some inode.(owner) /\ (F * inode_rep imap)%predicate (mem_union (fst s') (snd s'))) \/
+    (t = None /\ imap inum = None /\ (F * inode_rep imap)%predicate (mem_union (fst s') (snd s'))).
+Proof.
+  unfold get_block_numbers; intros; cleanup.
+  apply sp_bind in H.
+  simpl in *; cleanup.
+    
+  eapply sp_impl in H;
+  [> eapply get_inode_ok in H; eauto
+  |try solve [intros; cleanup; simpl; intuition eauto] ].
+  cleanup.
+  
+  + simpl in *; cleanup; left; eexists; intuition eauto.
+    eapply get_inode_ok in H0; eauto.
+    cleanup; eauto.
+    
+  + simpl in *; cleanup; right; intuition eauto.
+    eapply get_inode_ok in H0; eauto.
+    cleanup; eauto.
+Qed.
+
+Global Opaque alloc free extend change_owner get_block_number get_block_numbers get_owner.
