src/Noninterference/FileDiskNoninterference.v
@@ -1,6 +1,25 @@
 Require Import Framework FSParameters File FileDiskLayer FileDiskRefinement.
+Require Import AuthenticatedDiskLayer.
+Require Import TransactionalDiskLayer TransactionalDiskRefinement.
+Require Import TransactionCacheLayer.
+Require Import LoggedDiskLayer LoggedDiskRefinement.
+Require Import StorageLayer.
+Require Import CryptoDiskLayer CachedDiskLayer.
 
-Variable disk_size: nat.
+Notation "'CryptoDisk'" := CryptoDiskLang (at level 0).
+
+Notation "'CachedDisk'" := CachedDiskLang (at level 0).
+
+Notation "'LoggedDisk'" := LoggedDiskLang (at level 0).
+Notation "'LoggedDisk.refinement'" := LoggedDiskRefinement.
+
+Notation "'TransactionCache'" := TransactionCacheLang (at level 0).
+
+Notation "'TransactionalDisk'" := (TransactionalDiskLang data_length) (at level 0).
+Notation "'TransactionalDisk.refinement'" := TransactionalDiskRefinement.
+
+Notation "'AuthenticatedDisk'" := AuthenticatedDiskLang (at level 0).
+
 Notation "'FileDisk'" := (FileDiskLang inode_count) (at level 0).
 Notation "'FileDisk.refinement'" := FileDiskRefinement.
 
@@ -10,8 +29,7 @@ Definition same_for_user (s1 s2: FileDisk.(state)) :=
   let d1 := snd s1 in
   let d2 := snd s2 in
   u1 = u2 /\
-  addrs_match d1 d2 /\
-  addrs_match d2 d1 /\
+  addrs_match_exactly d1 d2 /\
   (forall inum file1 file2,
      d1 inum = Some file1 ->
      d2 inum = Some file2 ->
@@ -25,34 +43,6 @@ Definition same_for_user (s1 s2: FileDisk.(state)) :=
      length file1.(blocks) = length file2.(blocks)).
 
 (*
-
-Theorem self_simulation_from_wp :
-  forall O (L: Language O)
-    (valid_state: L.(state) -> Prop)
-    (valid_prog: forall T, L.(prog) T -> Prop)
-    (R: L.(state) -> L.(state) -> Prop), 
-
-    (forall T (p: L.(prog) T) (s1 s2: L.(state)) o s1' t1,
-       valid_state s1 ->
-       valid_state s2 ->
-       valid_prog T p ->
-       R s1 s2 ->
-       weakest_precondition L p (fun t' s' => R s1' s' /\ t' = t1) o s1 ->
-       exec L o s1 p (Finished s1' t1) ->
-       weakest_precondition L p (fun t' s' => R s1' s' /\ t' = t1) o s2) ->
-    SelfSimulation L valid_state valid_prog R.
-Proof.
-  intros.
-  constructor.
-  intros.
-  destruct s1'.
-  { (* Finished *)
-    eapply H in H3; eauto.
-    eapply wp_to_exec in H3; cleanup.
-    eexists; simpl; intuition eauto.
-    simpl.
- *)
-
 Theorem Invariant_for_file_disk_read:
   SelfSimulation FileDisk (fun _ => True) (fun T p => match p with
                                              | Op _ o =>
@@ -76,10 +66,11 @@ Proof.
       unfold same_for_user in *; cleanup.
       specialize (H1 a).
       destruct_fresh (snd s2 a); eauto; try congruence.
-      specialize (H3 a file f H9 D).
+      specialize (H2 a file f H9 D).
       setoid_rewrite H0 in H10.        
-      rewrite H3 in *; eauto.
+      rewrite H2 in *; eauto.
       repeat (econstructor; eauto; simpl).
+      destruct H1.
       exfalso; apply H1; eauto; setoid_rewrite H9; congruence.
     }          
     { (* Read Failed *)
@@ -92,22 +83,21 @@ Proof.
       -
         destruct_fresh (snd s2 a); eauto.
         unfold same_for_user in *; cleanup.
-        specialize (H3 a).
-        exfalso; eapply H3; try congruence; eauto.
+        specialize (H2 a); destruct H2.
+        exfalso; eapply H5; try congruence; eauto.
         eapply ExecReadFail; eauto.
       
       - unfold same_for_user in *; cleanup.
         specialize (H3 a).
         destruct_fresh (snd s2 a); eauto; try congruence.
-        specialize (H5 a file f H0 D).
-        specialize (H6 a file f H0 D); cleanup.
+        specialize (H4 a file f H0 D).
+        specialize (H5 a file f H0 D); cleanup.
         eapply ExecReadFail; eauto.
         right; right; intuition eauto.
         left; intuition; cleanup; eauto.
         right; apply nth_error_None.
-        rewrite <- H7; apply nth_error_None; eauto.
-        
-        exfalso; eapply H3; eauto;
+        rewrite <- H6; apply nth_error_None; eauto.        
+        destruct H3; exfalso; eapply H3; eauto;
         setoid_rewrite H0; congruence.
     }
   }
@@ -122,44 +112,665 @@ Proof.
   Unshelve.
   all: eauto.
 Qed.
+ *)
 
-Axiom self_simulation_for_file_disk:
-  SelfSimulation FileDisk (fun _ => True) (fun _ _ => True) same_for_user.
+Fixpoint horizontally_compose_valid_prog1 {O1 O2} (L1: Language O1) (L2: Language O2) (LL: Language (HorizontalComposition O1 O2)) C T (p1: prog L1 T) :=
+         match p1 with
+         | @Op _ T' p => C T' (Op (HorizontalComposition O1 O2) (P1 p))
+         | @Ret _ T' t => C T' (Ret t)
+         | @Bind _ T1 T2 p1 p2 =>
+           horizontally_compose_valid_prog1 L1 L2 LL C T1 p1 /\
+           (forall r, horizontally_compose_valid_prog1 L1 L2 LL C T2 (p2 r))
+         end.
+
+Fixpoint horizontally_compose_valid_prog2 {O1 O2} (L1: Language O1) (L2: Language O2) (LL: Language (HorizontalComposition O1 O2)) C T (p2: prog L2 T) :=
+         match p2 with
+         | @Op _ T' p => C T' (Op (HorizontalComposition O1 O2) (P2 p))
+         | @Ret _ T' t => C T' (Ret t)
+         | @Bind _ T1 T2 p1 p2 =>
+           horizontally_compose_valid_prog2 L1 L2 LL C T1 p1 /\
+           (forall r, horizontally_compose_valid_prog2 L1 L2 LL C T2 (p2 r))
+         end.
 
 
-Theorem ortsfr_file_disk:
-  oracle_refines_to_same_from_related FileDisk.refinement same_for_user.
+Lemma ss_hc_rev_p1:
+  forall O1 O2 (L1: Language O1) (L2: Language O2) (LL: Language (HorizontalComposition O1 O2))
+    R C V,
+    SelfSimulation LL R C V ->
+    forall s2,
+      SelfSimulation L1
+        (fun s1 => R (s1, s2))
+        (horizontally_compose_valid_prog1 L1 L2 LL C)
+        (fun s1 s1' =>  V (s1, s2) (s1', s2)).
 Proof.
-  unfold oracle_refines_to_same_from_related, refines_to_related.
-  induction p2; simpl; intros.
-  {
-    cleanup; eexists; intuition eauto.
-    unfold oracle_refines_to in *;
-    destruct p; cleanup.
-    { (* Read *)
-      unfold refines_to in *; cleanup.
-      eexists; split; eauto.
-      split_ors; cleanup.
-      + left; repeat eexists; eauto.
-        admit.
-      + right; repeat eexists; eauto.
-        admit.
-    }
-    { (* Write *)    
-      unfold refines_to in *; cleanup.
-      eexists; split; eauto.
-      unfold same_for_user in *; cleanup.
-      split_ors; cleanup.
-      +
-        split_ors; cleanup.
-        left; repeat eexists; left; intuition eauto.
-        admit.
-Abort.
+  intros.
+  constructor.
+  intros T o p.
+  generalize dependent s2.
+  generalize dependent o.
+  induction p; intros; cleanup.
+  - (* Op *)
+    repeat invert_exec; simpl in *.
+    + (* P1 Finished *)
+      edestruct H, self_simulation_correct.
+      apply H0.
+      apply H1.
+      all: simpl in *; eauto.
+      solve [repeat econstructor; eauto].
+      cleanup; simpl in *.
+      repeat invert_exec; simpl in *; cleanup; intuition.
+      exists (Finished s3 r0); intuition eauto.
       
-Theorem ecpv_file_disk:  
-exec_compiled_preserves_validity FileDisk.refinement                           
-   (refines_to_valid FileDisk.refinement (fun s => True)).
-Proof.
-  unfold exec_compiled_preserves_validity, refines_to_valid; intros; eauto.
+    + (* P1 Crashed *)
+      edestruct H, self_simulation_correct.
+      apply H0.
+      apply H1.
+      all: simpl in *; eauto.      
+      solve [repeat econstructor; eauto].
+      cleanup; simpl in *.
+      repeat invert_exec; simpl in *; cleanup; intuition.
+      exists (Crashed s3); intuition eauto.
+      repeat econstructor; eauto.
+
+  - (* Ret *)
+    invert_exec; cleanup;
+    eexists; simpl; intuition eauto; try solve [econstructor; eauto]; eauto.
+
+  - (* Bind *)
+    simpl in *; cleanup.
+    invert_exec; cleanup.
+    + (* Finished *)
+      edestruct IHp.
+      apply H1.
+      apply H2.
+      all: eauto.
+      cleanup; simpl in *.
+      destruct x3; simpl in *; intuition; cleanup.
+
+      edestruct H0.
+      apply H12.
+      apply H13.
+      all: eauto.
+      cleanup; simpl in *.
+      destruct x2; simpl in *; intuition; cleanup.
+
+      exists (Finished s4 t1); simpl; intuition eauto.
+      econstructor; eauto.
+
+    + split_ors; cleanup.
+      * (* p1 Crashed *)
+        edestruct IHp.
+        apply H1.
+        apply H2.
+        all: eauto.
+        cleanup; simpl in *.
+        destruct x1; simpl in *; intuition; cleanup.
+        exists (Crashed s3); simpl; intuition eauto.
+        solve [ econstructor; eauto].
+
+      * (* p2 crashed *)
+        edestruct IHp.
+        apply H1.
+        apply H2.
+        all: eauto.
+        cleanup; simpl in *.
+        destruct x3; simpl in *; intuition; cleanup.
+
+        edestruct H0.
+        apply H12.
+        apply H13.
+        all: eauto.
+        cleanup; simpl in *.
+        destruct x2; simpl in *; intuition; cleanup.
+        
+        exists (Crashed s4); simpl; intuition eauto.
+        econstructor; eauto.
 Qed.
 
+Lemma ss_hc_rev_p2:
+  forall O1 O2 (L1: Language O1) (L2: Language O2) (LL: Language (HorizontalComposition O1 O2))
+    R C V,
+    SelfSimulation LL R C V ->
+    forall s1,
+      SelfSimulation L2
+        (fun s2 => R (s1, s2))
+        (horizontally_compose_valid_prog2 L1 L2 LL C)
+        (fun s2 s2' =>  V (s1, s2) (s1, s2')).
+Proof.
+  intros.
+  constructor.
+  intros T o p.
+  generalize dependent s1.
+  generalize dependent o.
+  induction p; intros; cleanup.
+  - (* Op *)
+    repeat invert_exec; simpl in *.
+    + (* P2 Finished *)
+      edestruct H, self_simulation_correct.
+      apply H0.
+      apply H1.
+      all: simpl in *; eauto.
+      solve [repeat econstructor; eauto].
+      cleanup; simpl in *.
+      repeat invert_exec; simpl in *; cleanup; intuition.
+      exists (Finished s3 r0); intuition eauto.
+      
+    + (* P2 Crashed *)
+      edestruct H, self_simulation_correct.
+      apply H0.
+      apply H1.
+      all: simpl in *; eauto.      
+      solve [repeat econstructor; eauto].
+      cleanup; simpl in *.
+      repeat invert_exec; simpl in *; cleanup; intuition.
+      exists (Crashed s3); intuition eauto.
+      repeat econstructor; eauto.
+
+  - (* Ret *)
+    invert_exec; cleanup;
+    eexists; simpl; intuition eauto; try solve [econstructor; eauto]; eauto.
+
+  - (* Bind *)
+    simpl in *; cleanup.
+    invert_exec; cleanup.
+    + (* Finished *)
+      edestruct IHp.
+      apply H1.
+      apply H2.
+      all: eauto.
+      cleanup; simpl in *.
+      destruct x3; simpl in *; intuition; cleanup.
+
+      edestruct H0.
+      apply H12.
+      apply H13.
+      all: eauto.
+      cleanup; simpl in *.
+      destruct x2; simpl in *; intuition; cleanup.
+
+      exists (Finished s4 t1); simpl; intuition eauto.
+      econstructor; eauto.
+
+    + split_ors; cleanup.
+      * (* p1 Crashed *)
+        edestruct IHp.
+        apply H1.
+        apply H2.
+        all: eauto.
+        cleanup; simpl in *.
+        destruct x1; simpl in *; intuition; cleanup.
+        exists (Crashed s3); simpl; intuition eauto.
+        solve [ econstructor; eauto].
+
+      * (* p2 crashed *)
+        edestruct IHp.
+        apply H1.
+        apply H2.
+        all: eauto.
+        cleanup; simpl in *.
+        destruct x3; simpl in *; intuition; cleanup.
+
+        edestruct H0.
+        apply H12.
+        apply H13.
+        all: eauto.
+        cleanup; simpl in *.
+        destruct x2; simpl in *; intuition; cleanup.
+        
+        exists (Crashed s4); simpl; intuition eauto.
+        econstructor; eauto.
+Qed.
+
+Lemma ss_hc_rev:
+  forall O1 O2 (L1: Language O1) (L2: Language O2) (LL: Language (HorizontalComposition O1 O2))
+    R C V,
+    SelfSimulation LL R C V ->
+    (forall s2,
+      SelfSimulation L1
+        (fun s1 => R (s1, s2))
+        (horizontally_compose_valid_prog1 L1 L2 LL C)
+        (fun s1 s1' =>  V (s1, s2) (s1', s2))) /\
+    (forall s1,
+      SelfSimulation L2
+        (fun s2 => R (s1, s2))
+        (horizontally_compose_valid_prog2 L1 L2 LL C)
+        (fun s2 s2' =>  V (s1, s2) (s1, s2'))).
+Proof.
+  intros; split; intros.
+  eapply ss_hc_rev_p1; eauto.
+  eapply ss_hc_rev_p2; eauto.
+Qed.
+
+Lemma ss_impl:
+  forall O (L: Language O)
+    R1 (R2: state L -> Prop) C1 (C2: forall T, prog L T -> Prop) V1 (V2: state L -> state L -> Prop),
+    SelfSimulation L R1 C1 V1 ->
+    (forall s, R1 s <-> R2 s) ->
+    (forall T p, C1 T p <-> C2 T p) ->
+    (forall s s', V1 s s' <-> V2 s s') ->
+    SelfSimulation L R2 C2 V2.
+Proof.
+  intros; constructor; intros.
+  edestruct H, self_simulation_correct.
+  eapply H0; apply H3.
+  eapply H0; apply H4.
+  eapply H1; eauto.
+  eauto.
+  eapply H2; eauto.
+  cleanup.
+  eexists; intuition eauto.
+  eapply H2; eauto.
+  eapply H0; eauto.
+  eapply H0; eauto.
+Qed.
+
+Lemma ss_hc:
+  forall O1 O2 (L1: Language O1) (L2: Language O2) (LL: Language (HorizontalComposition O1 O2))
+  R1 R2 C1 C2 V1 V2,
+  SelfSimulation L1 R1 C1 V1 ->
+  SelfSimulation L2 R2 C2 V2 ->
+  SelfSimulation LL
+      (fun s => R1 (fst s) /\ R2 (snd s))
+      (fix CH T p :=
+         match p with
+         | Op _ (@P1 _ _ T1 p0) => C1 T1 (Op _ p0)
+         | Op _ (@P2 _ _ T1 p0) => C2 T1 (Op _ p0)
+         | @Ret _ T0 t => True
+         | @Bind _ T1 T2 p1 p2 => CH T1 p1 /\ (forall r, CH T2 (p2 r))
+         end)
+      (fun s s' => V1 (fst s) (fst s') /\ V2 (snd s) (snd s')).
+Proof.
+  intros.
+  constructor.
+  intros T o p.
+  generalize dependent o.
+  induction p; intros.
+  - (* Op *)
+    destruct p; simpl in *; cleanup;
+    repeat invert_exec; simpl in *.
+    + (* P1 Finished *)
+      edestruct H, self_simulation_correct.
+      apply H1.
+      apply H2.
+      eauto.      
+      econstructor; eauto.
+      eauto.
+      cleanup; simpl in *.
+      invert_exec; simpl in *; cleanup; intuition.
+      exists (Finished (s', snd s2) r0); intuition eauto.
+      repeat econstructor; eauto.
+      
+    + (* P1 Crashed *)
+      edestruct H, self_simulation_correct.
+      apply H1.
+      apply H2.
+      eauto.      
+      solve [econstructor; eauto].
+      eauto.
+      cleanup; simpl in *.
+      invert_exec; simpl in *; cleanup; intuition.
+      exists (Crashed (s', snd s2)); intuition eauto.
+      repeat econstructor; eauto.
+
+    + (* P2 Finished *)
+      edestruct H0, self_simulation_correct.
+      apply H8.
+      apply H7.
+      eauto.      
+      econstructor; eauto.
+      eauto.
+      cleanup; simpl in *.
+      invert_exec; simpl in *; cleanup; intuition.
+      exists (Finished (fst s2, s') r0); intuition eauto.
+      repeat econstructor; eauto.
+
+    + (* P2 Crashed *)
+      edestruct H0, self_simulation_correct.
+      apply H8.
+      apply H7.
+      eauto.      
+      solve [econstructor; eauto].
+      eauto.
+      cleanup; simpl in *.
+      invert_exec; simpl in *; cleanup; intuition.
+      exists (Crashed (fst s2, s')); intuition eauto.
+      repeat econstructor; eauto.
+
+  - (* Ret *)
+    invert_exec; cleanup;
+    eexists; simpl; intuition eauto; try solve [econstructor; eauto]; eauto.
+
+  - (* Bind *)
+    invert_exec; cleanup.
+    + (* Finished *)
+      edestruct IHp.
+      split; [apply H2 | apply H12].
+      split; [apply H3 | apply H11].
+      eauto.
+      eauto.
+      eauto.
+      cleanup; simpl in *.
+      destruct x3; simpl in *; intuition; cleanup.
+
+      edestruct H1.
+      split; [apply H16 | apply H19].
+      split; [apply H17 | apply H18].
+      eapply H10.
+      eauto.
+      eauto.
+      cleanup; simpl in *.
+      destruct x2; simpl in *; intuition; cleanup.
+
+      exists (Finished s3 t1); simpl; intuition eauto.
+      econstructor; eauto.
+
+    + split_ors; cleanup.
+      * (* p1 Crashed *)
+        edestruct IHp.
+        split; [apply H2 | apply H11].
+        split; [apply H3 | apply H10].
+        eauto.
+        eauto.
+        eauto.
+        cleanup; simpl in *.
+        destruct x1; simpl in *; intuition; cleanup.
+        exists (Crashed s0); simpl; intuition eauto.
+        solve [ econstructor; eauto].
+
+      * (* p2 crashed *)
+        edestruct IHp.
+        split; [apply H2 | apply H11].
+        split; [apply H3 | apply H10].
+        eauto.
+        eauto.
+        eauto.
+        cleanup; simpl in *.
+        destruct x3; simpl in *; intuition; cleanup.
+        
+        edestruct H1.
+        split; [apply H16 | apply H19].
+        split; [apply H17 | apply H18].
+        eapply H9.
+        eauto.
+        eauto.
+        cleanup; simpl in *.
+        destruct x2; simpl in *; intuition; cleanup.
+        
+        exists (Crashed s3); simpl; intuition eauto.
+        econstructor; eauto.
+Qed.
+
+(** Relation Definitions *)
+
+(** Top Layer *)
+(* File Disk *)
+Definition FD_valid_state := fun (s: state FileDisk) => exists fmap, files_rep fmap (snd s).
+Definition FD_valid_prog  := fun T (p: prog FileDisk T) => True.
+Definition FD_related_states := same_for_user.
+
+(** Intermediate Layers *)
+(* Authenticated Disk *)
+Definition AD_valid_state := refines_to_valid FileDisk.refinement FD_valid_state.
+Definition AD_valid_prog  := compiles_to_valid FileDisk.refinement FD_valid_prog.
+Definition AD_related_states := refines_to_related FileDisk.refinement FD_related_states.
+
+(* Transactional Disk *)
+Definition TD_valid_state s1 := fun s2 => AD_valid_state (s1, s2).
+Definition TD_valid_prog  := horizontally_compose_valid_prog2 AuthenticationLang TransactionalDisk AuthenticatedDisk AD_valid_prog.
+Definition TD_related_states s1 := fun s2 s2' => AD_related_states (s1, s2) (s1, s2').
+
+(* Transaction Cache *)
+Definition TC_valid_state s1 := refines_to_valid TransactionalDisk.refinement (TD_valid_state s1).
+Definition TC_valid_prog  := compiles_to_valid TransactionalDisk.refinement TD_valid_prog.
+Definition TC_related_states s1 := refines_to_related TransactionalDisk.refinement (TD_related_states s1).
+
+(* Logged Disk *)
+Definition LD_valid_state s := fun s2 => TC_valid_state (fst s) (snd s, s2).
+Definition LD_valid_prog  := horizontally_compose_valid_prog2 (StorageLang (list (addr * value))) LoggedDisk TransactionCache TC_valid_prog.
+Definition LD_related_states s := fun s2 s2' => TC_related_states (fst s) (snd s, s2) (snd s, s2').
+
+(* Cached Disk *)
+Definition CD_valid_state s1 := refines_to_valid LoggedDisk.refinement (LD_valid_state s1).
+Definition CD_valid_prog  := compiles_to_valid LoggedDisk.refinement LD_valid_prog.
+Definition CD_related_states s1 := refines_to_related LoggedDisk.refinement (LD_related_states s1).
+
+(* Crypto Disk *)
+Definition CrD_valid_state s := fun s2 => CD_valid_state (fst s) (snd s, s2).
+Definition CrD_valid_prog  := horizontally_compose_valid_prog2 (CacheLang addr_dec value) CryptoDisk CachedDisk CD_valid_prog.
+Definition CrD_related_states s := fun s2 s2' => CD_related_states (fst s) (snd s, s2) (snd s, s2').
+
+(** Bottom Layers *)
+(* Authentication Layer *)
+Definition AL_valid_state s2 := fun s1 => AD_valid_state (s1, s2).
+Definition AL_valid_prog  := horizontally_compose_valid_prog1 AuthenticationLang TransactionalDisk AuthenticatedDisk AD_valid_prog.
+Definition AL_related_states s2 := fun s1 s1' => AD_related_states (s1, s2) (s1', s2).
+
+(* Storage Layer *)
+Definition SL_valid_state s := fun s1 => TC_valid_state (fst s) (s1, snd s).
+Definition SL_valid_prog  := horizontally_compose_valid_prog1 (StorageLang (list (addr * value))) LoggedDisk TransactionCache TC_valid_prog.
+Definition SL_related_states s := fun s1 s1' => TC_related_states (fst s) (s1, snd s) (s1', snd s).
+
+(* Cache Layer *)
+Definition CL_valid_state s := fun s1 => CD_valid_state (fst s) (s1, snd s).
+Definition CL_valid_prog  := horizontally_compose_valid_prog1 (CacheLang addr_dec value) CryptoDisk CachedDisk CD_valid_prog.
+Definition CL_related_states s := fun s1 s1' => CD_related_states (fst s) (s1, snd s) (s1', snd s).
+
+(* Crypto Layer *)
+Definition CrL_valid_state s := fun s1 => CrD_valid_state (fst s) (s1, snd s).
+Definition CrL_valid_prog  := horizontally_compose_valid_prog1 CryptoLang (DiskLang addr_dec value) CryptoDisk CrD_valid_prog.
+Definition CrL_related_states s := fun s1 s1' =>  CrD_related_states (fst s) (s1, snd s) (s1', snd s).
+
+(* Disk Layer *)
+Definition DL_valid_state s := fun s2 => CrD_valid_state (fst s) (snd s, s2).
+Definition DL_valid_prog  := horizontally_compose_valid_prog2 CryptoLang (DiskLang addr_dec value) CryptoDisk CrD_valid_prog.
+Definition DL_related_states s := fun s2 s2' => CrD_related_states (fst s) (snd s, s2) (snd s, s2').
+
+
+
+(** NI Theorems *)
+(** Top Layer *)
+Theorem ss_FD:
+  SelfSimulation FileDisk FD_valid_state FD_valid_prog FD_related_states.
+Proof. Admitted.
+
+(** Intermediate Layers *)
+Theorem ss_AD:
+  SelfSimulation AuthenticatedDisk AD_valid_state AD_valid_prog AD_related_states.
+Proof.
+  intros.
+  unfold AD_valid_state, AD_valid_prog, AD_related_states; simpl.   
+  (* Theorem from file disk refinement here *)
+Admitted.
+
+Theorem ss_TD:
+  forall s, SelfSimulation TransactionalDisk (TD_valid_state s) TD_valid_prog (TD_related_states s).
+Proof.
+  intros.
+  unfold TD_valid_state, TD_valid_prog, TD_related_states; simpl.  
+  eapply ss_hc_rev_p2 with (R:= AD_valid_state) (V:= AD_related_states).
+  apply ss_AD.
+Qed.
+
+Theorem ss_TC:
+  forall s, SelfSimulation TransactionCache (TC_valid_state s) TC_valid_prog (TC_related_states s).
+Proof.
+  intros.
+  unfold TC_valid_state, TC_valid_prog, TC_related_states; simpl.
+  (* Theorem from transactional disk refinement here *)
+Admitted.
+
+Theorem ss_LD:
+  forall s, SelfSimulation LoggedDisk (LD_valid_state s) LD_valid_prog (LD_related_states s).
+Proof.
+  intros.
+  unfold LD_valid_state, LD_valid_prog, LD_related_states; simpl.
+  eapply ss_hc_rev_p2 with (R:= TC_valid_state (fst s)) (V:= TC_related_states (fst s)).
+  eapply ss_TC.
+Qed.
+
+Theorem ss_CD:
+  forall s, SelfSimulation CachedDisk (CD_valid_state s) CD_valid_prog (CD_related_states s).
+Proof.
+  intros.
+  unfold CD_valid_state, CD_valid_prog, CD_related_states; simpl.
+  (* Need theorem from logged disk refinement here *)
+Admitted.
+
+Theorem ss_CrD:
+  forall s, SelfSimulation CryptoDisk (CrD_valid_state s) CrD_valid_prog (CrD_related_states s).
+Proof.
+  intros.
+  unfold CrD_valid_state, CrD_valid_prog, CrD_related_states; simpl.
+  eapply ss_hc_rev_p2 with (R:= CD_valid_state (fst s)) (V:= CD_related_states (fst s)).
+  eapply ss_CD.
+Qed.
+
+(** Bottom Layers *)
+Theorem ss_AL:
+  forall s, SelfSimulation (AuthenticationLang) (AL_valid_state s) AL_valid_prog (AL_related_states s).
+Proof.
+  intros.
+  unfold AL_valid_state, AL_valid_prog, AL_related_states; simpl.  
+  eapply ss_hc_rev_p1 with (R:= AD_valid_state) (V:= AD_related_states).
+  apply ss_AD.
+Qed.
+
+Theorem ss_SL:
+  forall s, SelfSimulation (StorageLang (list (addr * value))) (SL_valid_state s) SL_valid_prog (SL_related_states s).
+Proof.
+  intros.
+  unfold SL_valid_state, SL_valid_prog, SL_related_states; simpl.
+  eapply ss_hc_rev_p1 with (R:= TC_valid_state (fst s)) (V:= TC_related_states (fst s)).
+  eapply ss_TC.
+Qed.
+
+
+Theorem ss_CL:
+  forall s, SelfSimulation (CacheLang addr_dec value) (CL_valid_state s) CL_valid_prog (CL_related_states s).
+Proof.
+  intros.
+  unfold CL_valid_state, CL_valid_prog, CL_related_states; simpl.
+  eapply ss_hc_rev_p1 with (R:= CD_valid_state (fst s)) (V:= CD_related_states (fst s)).
+  eapply ss_CD.
+Qed.
+
+Theorem ss_DL:
+  forall s, SelfSimulation (DiskLang addr_dec value) (DL_valid_state s) DL_valid_prog (DL_related_states s).
+Proof.
+  intros.
+  unfold DL_valid_state, DL_valid_prog, DL_related_states; simpl.  
+  eapply ss_hc_rev_p2 with (R:= CrD_valid_state (fst s)) (V:= CrD_related_states (fst s)).
+  eapply ss_CrD.
+Qed.
+
+Theorem ss_CrL:
+  forall s, SelfSimulation CryptoLang (CrL_valid_state s) CrL_valid_prog (CrL_related_states s).
+Proof.
+  intros.  
+  unfold CrL_valid_state, CrL_valid_prog, CrL_related_states; simpl.  
+  eapply ss_hc_rev_p1 with (R:= CrD_valid_state (fst s)) (V:= CrD_related_states (fst s)).
+  eapply ss_CrD.
+Qed.
+
+
+(** Required theorems for transfer *)
+Theorem ortsfr_FD:
+  oracle_refines_to_same_from_related FileDisk.refinement FD_related_states.
+Proof. Admitted.
+
+Theorem ecpv_FD:  
+exec_compiled_preserves_validity FileDisk.refinement AD_valid_state.
+Proof.
+  unfold AD_valid_state, FD_valid_state,
+  exec_compiled_preserves_validity, refines_to_valid; intros; eauto.
+Qed.
+
+
+Theorem ortsfr_TD:
+  forall s, oracle_refines_to_same_from_related TransactionalDisk.refinement (TD_related_states s).
+Proof.
+  unfold oracle_refines_to_same_from_related; simpl.
+  induction p2; simpl; intros.
+  cleanup.
+  eexists; intuition eauto.
+  
+  - destruct p; simpl in *.
+    { (* Start *)
+      split_ors; cleanup.
+      { (* Finished *)
+        destruct sbs.
+        edestruct wp_to_exec with (p:= Transaction.start)
+      (Q:= strongest_postcondition TransactionToTransactionalDisk.Definitions.low Transaction.start
+         (fun o' s' => refines_to_related TransactionalDisk.refinement (TD_related_states s) s1 s' /\ s' = s2 /\ o' = o)); eauto.
+        simpl.
+        do 2 eexists; intuition eauto; simpl.
+        eexists; intuition eauto; simpl.
+        eexists; intuition eauto; simpl.
+        eexists; intuition eauto; simpl.
+        eexists; intuition eauto; simpl.
+        instantiate (1:= s2);
+        instantiate (1:= fst s2); simpl; eauto.
+        destruct s2; eauto.
+        
+        eapply exec_to_sp with (P:= fun o' s' => refines_to_related TransactionalDisk.refinement (TD_related_states s) s' s2 /\ s' = s1 /\ o' = o) in H0; eauto.
+        simpl in *; cleanup; eauto.
+      
+      simpl; eauto.
+      cleanup.
+      simpl in H2; cleanup.
+      left; do 2 eexists; intuition eauto.
+      destruct x; simpl in *; cleanup; eauto.
+    + split_ors; cleanup.
+       edestruct wcp_to_exec with (p:= Transaction.start)
+      (Q:= strongest_crash_postcondition TransactionToTransactionalDisk.Definitions.low Transaction.start
+         (fun o' s' =>
+            refines_to_related TransactionalDisk.refinement (TD_related_states s) s1 s' /\ s' = s2 /\ o' = o)); eauto.
+       do 2 eexists; intuition eauto; simpl.
+
+       eapply exec_to_scp with (P:= fun o' s' => refines_to_related TransactionalDisk.refinement (TD_related_states s) s' s2 /\ s' = s1 /\ o' = o) in H0; eauto.
+       simpl in *; cleanup; eauto.
+
+       split_ors; cleanup; simpl in *;
+       try match goal with
+       | [H: StorageLayer.strongest_crash_postcondition' _ _ _ |- _ ] =>
+         inversion H; clear H; cleanup
+       end.
+
+      left.
+      eexists; intuition eauto; simpl.
+      eexists; intuition eauto; simpl.
+      eexists; intuition eauto; simpl.
+      left.
+      eexists; intuition eauto; simpl.
+      instantiate (1:= s2);
+      simpl; eauto.
+      destruct s2; eauto.
+
+      right.
+      eexists; intuition eauto; simpl.
+      eexists; intuition eauto; simpl.
+      repeat econstructor.
+      econstructor.
+      solve [repeat econstructor; eauto].
+      eexists; intuition eauto; simpl.
+      left.
+      eexists; intuition eauto; simpl.
+      instantiate (1:= s2);
+      simpl; eauto.
+      destruct s2; eauto.
+
+      
+      
+      
+      simpl; eauto.
+      cleanup.
+      simpl in H2; cleanup.
+      left; do 2 eexists; intuition eauto.
+      destruct x; simpl in *; cleanup; eauto.
+
+      
+      econstructor.
+
+
+      
+Admitted.
