src/Framework/Simulation/Metatheory.v
@@ -50,6 +50,7 @@ Proof.
       eapply_fresh H in H0; cleanup; clear H H1
   end.
 
+
   match goal with
   | [H: refines_to_valid _ _ ?s,
      H0: refines_to _ ?s _,
@@ -80,13 +81,6 @@ Proof.
   end.  
   
   do 2 eexists; intuition eauto.
-  do 2 (eapply result_same_transitive; eauto).
-  apply result_same_symmetric; auto.
-  
-  repeat match goal with
-  | [H: forall _, extract_ret _ ?a = _ |- extract_ret _ ?a = _] =>
-    rewrite H; auto
-         end.
 
   match goal with
   |[ H0: oracle_refines_to_same_from_related _ _ |- _] =>
@@ -94,6 +88,136 @@ Proof.
   end.
   unfold refines_to_related; eauto. 
 Qed.
+
+Local Theorem bisimulation_to_comp_preserve:
+  forall OL OH (LL: Language OL) (LH: Language OH) (R: Refinement LL LH),
+    StrongBisimulation R ->
+    forall T (p1 p2: LH.(prog) T),
+       R.(compile) p1 = R.(compile) p2 ->
+       (forall s o1 o2, R.(oracle_refines_to) s p1 o1 o2 -> R.(oracle_refines_to) s p2 o1 o2) ->
+       (forall o s ret1 ret2,
+          (exists s1 o1, R.(refines_to) s1 s /\
+          R.(oracle_refines_to) s1 p1 o1 o) ->
+          exec LH o s p1 ret1 ->
+          exec LH o s p2 ret2 ->
+          extract_ret ret1 = extract_ret ret2 /\
+          exists s1', refines_to R s1'(extract_state ret1) /\
+                 refines_to R s1'(extract_state ret2)).
+Proof.
+  intros.
+  destruct H; cleanup.
+  match goal with
+  | [H: refines_to _ _ s |- _] =>
+    eapply_fresh strong_bisimulation_correct in H; eauto; cleanup
+  end.
+
+  match goal with
+    | [H: forall _, exec LL _ _ _ _ -> _,
+       H0: exec LH _ _ _ _,
+       H1: forall _, exec LH _ _ _ _ -> _ |- _] =>
+      eapply_fresh H1 in H0; cleanup; clear H H1
+  end.
+
+  match goal with
+  | [H: refines_to _ _ s |- _] =>
+    eapply_fresh strong_bisimulation_correct in H
+  end.
+
+  2: apply H1; eauto.
+  cleanup.
+  match goal with
+    | [H: forall _, exec LL _ _ _ _ -> _,
+       H0: exec LL _ _ _ _,
+       H1: forall _, exec LH _ _ _ _ -> _ |- _] =>
+      eapply_fresh H in H0; cleanup; clear H H1
+  end.
+
+  destruct ret1, ret2, x1, x2; simpl in *; cleanup;
+  eapply exec_deterministic_wrt_oracle in H4; eauto; cleanup;
+  intuition eauto; cleanup; eauto.
+Qed.
+  
+
+Theorem transfer_high_to_low_secret:
+  forall OL OH (LL: Language OL) (LH: Language OH) (R: Refinement LL LH)
+    related_states_h
+    valid_state_h
+    valid_prog_h
+    T T' (p: T -> LH.(prog) T'),
+    
+    SelfSimulationForSecretInputs
+      LH
+      valid_state_h
+      valid_prog_h
+      related_states_h p ->
+    
+    StrongBisimulation R ->
+
+    high_oracle_exists R ->
+
+    (** We need compilation validity **)
+    (forall T (p1 p2: LH.(prog) T),
+       compile R p1 = compile R p2 ->
+       valid_prog_h T p1 ->
+       valid_prog_h T p2) ->
+         
+    (** 
+        We need oracle refinement being invariant on high input.
+        Merge this with oracle_refines_to_same_from_related 
+        to get a statement that says
+        "Oracle refinement is invariant on secrets." 
+     **)
+    (forall s t1 t2 o1 o2, R.(oracle_refines_to) s (p t1) o1 o2 -> R.(oracle_refines_to) s (p t2) o1 o2) ->
+    
+    SelfSimulationForSecretInputs
+      LL
+      (fun s => exists s', R.(refines_to) s s' /\ valid_state_h s')
+      (compiles_to_valid R valid_prog_h)
+      (refines_to_related R related_states_h)
+      (fun t => R.(compile) (p t)).
+Proof.
+  unfold SelfSimulationForSecretInputs, refines_to_related, compiles_to_valid; intros.
+  pose proof bisimulation_to_comp_preserve  as Hx.
+  specialize Hx with (1:=H0).
+  destruct H0; cleanup.
+
+  rewrite <- H5 in H7. 
+  match goal with
+  | [H: high_oracle_exists _,
+     H0: exec LL _ _ _ _ |- _] =>
+    pose proof H; edestruct H; try apply H0; eauto
+  end.
+
+  match goal with
+  | [H: refines_to _ s _ |- _] =>
+    eapply_fresh strong_bisimulation_correct in H; eauto; cleanup
+  end.
+
+  match goal with
+    | [H: forall _, exec LL _ _ _ _ -> _,
+       H0: exec LL _ _ _ _,
+       H1: forall _, exec LH _ _ _ _ -> _ |- _] =>
+      eapply_fresh H in H0; cleanup; clear H H1
+  end.
+
+  eapply H in H10; try apply H9; eauto; cleanup.
+  
+  match goal with
+  | [H: exec LH _ ?x2 _ _,
+     H1: refines_to _ ?s2 ?x2  |- _] =>
+      eapply_fresh strong_bisimulation_correct in H; eauto; cleanup
+  end.
+  
+  eexists; intuition eauto.
+Qed.
+
+
+
+
+
+
+
+
 
 (*
 Theorem transfer_high_to_low_for_valid_states :
